theories/rules/rules_Jnz.v
@@ -233,7 +233,7 @@ Section cap_lang_rules.
   Lemma wp_jnz_success_next E r1 r2 pc_p pc_b pc_e pc_a pc_a' w w1 :
     decodeInstrW w = Jnz r1 r2 →
     isCorrectPC (WCap pc_p pc_b pc_e pc_a) →
-    (pc_a + 1)%a = Some pc_a' →
+    (pc_a + 1)%va = Some pc_a' →
 
     {{{ ▷ PC ↦ᵣ WCap pc_p pc_b pc_e pc_a
         ∗ ▷ (TEMP_virt_to_phys pc_a) ↦ₐ w
