theories/rules/rules_Mov.v
@@ -89,7 +89,7 @@ Section cap_lang_rules.
   Lemma wp_move_success_z E pc_p pc_b pc_e pc_a pc_a' w r1 wr1 z :
     decodeInstrW w = Mov r1 (inl z) →
     isCorrectPC (WCap pc_p pc_b pc_e pc_a) →
-    (pc_a + 1)%a = Some pc_a' →
+    (pc_a + 1)%va = Some pc_a' →
 
     {{{ ▷ PC ↦ᵣ WCap pc_p pc_b pc_e pc_a
         ∗ ▷ (TEMP_virt_to_phys pc_a) ↦ₐ w
@@ -118,7 +118,7 @@ Section cap_lang_rules.
   Lemma wp_move_success_reg E pc_p pc_b pc_e pc_a pc_a' w r1 wr1 rv wrv :
     decodeInstrW w = Mov r1 (inr rv) →
     isCorrectPC (WCap pc_p pc_b pc_e pc_a) →
-    (pc_a + 1)%a = Some pc_a' →
+    (pc_a + 1)%va = Some pc_a' →
 
     {{{ ▷ PC ↦ᵣ WCap pc_p pc_b pc_e pc_a
         ∗ ▷ (TEMP_virt_to_phys pc_a) ↦ₐ w
@@ -149,7 +149,7 @@ Section cap_lang_rules.
   Lemma wp_move_success_reg_same E pc_p pc_b pc_e pc_a pc_a' w r1 wr1 :
     decodeInstrW w = Mov r1 (inr r1) →
     isCorrectPC (WCap pc_p pc_b pc_e pc_a) →
-    (pc_a + 1)%a = Some pc_a' →
+    (pc_a + 1)%va = Some pc_a' →
 
     {{{ ▷ PC ↦ᵣ WCap pc_p pc_b pc_e pc_a
         ∗ ▷ (TEMP_virt_to_phys pc_a) ↦ₐ w
@@ -178,7 +178,7 @@ Section cap_lang_rules.
   Lemma wp_move_success_reg_samePC E pc_p pc_b pc_e pc_a pc_a' w :
     decodeInstrW w = Mov PC (inr PC) →
     isCorrectPC (WCap pc_p pc_b pc_e pc_a) →
-    (pc_a + 1)%a = Some pc_a' →
+    (pc_a + 1)%va = Some pc_a' →
 
     {{{ ▷ PC ↦ᵣ WCap pc_p pc_b pc_e pc_a
         ∗ ▷ (TEMP_virt_to_phys pc_a) ↦ₐ w }}}
@@ -204,7 +204,7 @@ Section cap_lang_rules.
   Lemma wp_move_success_reg_toPC E pc_p pc_b pc_e pc_a w r1 p b e a a':
     decodeInstrW w = Mov PC (inr r1) →
     isCorrectPC (WCap pc_p pc_b pc_e pc_a) →
-    (a + 1)%a = Some a' →
+    (a + 1)%va = Some a' →
 
     {{{ ▷ PC ↦ᵣ WCap pc_p pc_b pc_e pc_a
         ∗ ▷ (TEMP_virt_to_phys pc_a) ↦ₐ w
@@ -233,7 +233,7 @@ Section cap_lang_rules.
   Lemma wp_move_success_reg_fromPC E pc_p pc_b pc_e pc_a pc_a' w r1 wr1 :
     decodeInstrW w = Mov r1 (inr PC) →
     isCorrectPC (WCap pc_p pc_b pc_e pc_a) →
-    (pc_a + 1)%a = Some pc_a' →
+    (pc_a + 1)%va = Some pc_a' →
 
     {{{ ▷ PC ↦ᵣ WCap pc_p pc_b pc_e pc_a
         ∗ ▷ (TEMP_virt_to_phys pc_a) ↦ₐ w
