theories/rules/rules_Seal.v
@@ -27,13 +27,13 @@ Section cap_lang_rules.
   | Seal_fail_bounds w p b e a sb:
       regs !! src1 = Some (WSealRange p b e a) →
       regs !! src2 = Some (WSealable sb) →
-      (permit_seal p = false ∨ withinBoundsVirt b e a = false) →
+      (permit_seal p = false ∨ withinBounds b e a = false) →
       Seal_failure regs dst src1 src2 regs
   | Seal_fail_incrPC p b e a sb :
       regs !! src1 = Some (WSealRange p b e a) →
       regs !! src2 = Some (WSealable sb) →
       permit_seal p = true →
-      withinBoundsVirt b e a = true →
+      withinBounds b e a = true →
       incrementPC (<[ dst := WSealed a sb ]> regs) = None →
       Seal_failure regs dst src1 src2 regs.
 
@@ -42,7 +42,7 @@ Section cap_lang_rules.
       regs !! src1 = Some (WSealRange p b e a) →
       regs !! src2 = Some (WSealable sb) →
       permit_seal p = true →
-      withinBoundsVirt b e a = true →
+      withinBounds b e a = true →
       incrementPC (<[ dst := WSealed a sb ]> regs) = Some regs' →
       Seal_spec regs dst src1 src2 regs' NextIV
   | Seal_spec_failure :
@@ -106,7 +106,7 @@ Section cap_lang_rules.
      }
      destruct r2v as [ | sb | ]; try inversion Hr2v. clear Hr2v.
 
-     destruct (permit_seal p && withinBoundsVirt b e a) eqn:HSA.
+     destruct (permit_seal p && withinBounds b e a) eqn:HSA.
      2 : { (* Failure: r2 is either not within bounds or doesnt allow sealing *)
        symmetry in Hstep; inversion Hstep; clear Hstep. subst c σ2.
        apply andb_false_iff in HSA.
@@ -148,8 +148,8 @@ Section cap_lang_rules.
     decodeInstrW w = Seal dst r1 r2 →
     isCorrectPC (WCap pc_p pc_b pc_e pc_a) →
     permit_seal p = true →
-    withinBoundsVirt b e a = true →
-    (pc_a + 1)%a = Some pc_a' →
+    withinBounds b e a = true →
+    (pc_a + 1)%va = Some pc_a' →
 
     {{{ ▷ PC ↦ᵣ WCap pc_p pc_b pc_e pc_a
         ∗ ▷ (TEMP_virt_to_phys pc_a) ↦ₐ w
@@ -188,8 +188,8 @@ Section cap_lang_rules.
     decodeInstrW w = Seal r1 r1 r2 →
     isCorrectPC (WCap pc_p pc_b pc_e pc_a) →
     permit_seal p = true →
-    withinBoundsVirt b e a = true →
-    (pc_a + 1)%a = Some pc_a' →
+    withinBounds b e a = true →
+    (pc_a + 1)%va = Some pc_a' →
 
     {{{ ▷ PC ↦ᵣ WCap pc_p pc_b pc_e pc_a
         ∗ ▷ (TEMP_virt_to_phys pc_a) ↦ₐ w
@@ -225,8 +225,8 @@ Section cap_lang_rules.
     decodeInstrW w = Seal r2 r1 r2 →
     isCorrectPC (WCap pc_p pc_b pc_e pc_a) →
     permit_seal p = true →
-    withinBoundsVirt b e a = true →
-    (pc_a + 1)%a = Some pc_a' →
+    withinBounds b e a = true →
+    (pc_a + 1)%va = Some pc_a' →
 
     {{{ ▷ PC ↦ᵣ WCap pc_p pc_b pc_e pc_a
         ∗ ▷ (TEMP_virt_to_phys pc_a) ↦ₐ w
@@ -264,8 +264,8 @@ Section cap_lang_rules.
     decodeInstrW w = Seal dst r1 PC →
     isCorrectPC (WCap pc_p pc_b pc_e pc_a) →
     permit_seal p = true →
-    withinBoundsVirt b e a = true →
-    (pc_a + 1)%a = Some pc_a' →
+    withinBounds b e a = true →
+    (pc_a + 1)%va = Some pc_a' →
 
     {{{ ▷ PC ↦ᵣ WCap pc_p pc_b pc_e pc_a
         ∗ ▷ (TEMP_virt_to_phys pc_a) ↦ₐ w
@@ -301,8 +301,8 @@ Section cap_lang_rules.
     decodeInstrW w = Seal r1 r1 PC →
     isCorrectPC (WCap pc_p pc_b pc_e pc_a) →
     permit_seal p = true →
-    withinBoundsVirt b e a = true →
-    (pc_a + 1)%a = Some pc_a' →
+    withinBounds b e a = true →
+    (pc_a + 1)%va = Some pc_a' →
 
     {{{ ▷ PC ↦ᵣ WCap pc_p pc_b pc_e pc_a
         ∗ ▷ (TEMP_virt_to_phys pc_a) ↦ₐ w
@@ -335,7 +335,7 @@ Section cap_lang_rules.
   Lemma wp_seal_nosb_r2 E pc_p pc_b pc_e pc_a w r1 r2 p b e a w2 pc_a' :
     decodeInstrW w = Seal r2 r1 r2 →
     isCorrectPC (WCap pc_p pc_b pc_e pc_a) →
-    (pc_a + 1)%a = Some pc_a' →
+    (pc_a + 1)%va = Some pc_a' →
     is_sealb w2 = false →
 
     {{{ ▷ PC ↦ᵣ WCap pc_p pc_b pc_e pc_a
