theories/rules_binary/rules_binary_Store.v
@@ -28,15 +28,15 @@ Section cap_lang_spec_rules.
    isCorrectPC (WCap pc_p pc_b pc_e pc_a) →
    regs !! PC = Some (WCap pc_p pc_b pc_e pc_a) →
    regs_of (Store r1 r2) ⊆ dom regs →
-   mem !! pc_a = Some w →
+   mem !! (TEMP_virt_to_phys pc_a) = Some w →
    allow_store_map_or_true r1 regs mem →
    nclose specN ⊆ Ep →
 
-   spec_ctx ∗ ⤇ fill K (Instr Executable) ∗ (▷ [∗ map] a↦w ∈ mem, a ↣ₐ w) ∗ (▷ [∗ map] k↦y ∈ regs, k ↣ᵣ y)
+   spec_ctx ∗ ⤇ fill K (Instr Executable) ∗ (▷ [∗ map] (a:PhysAddr)↦w ∈ mem, a ↣ₐ w) ∗ (▷ [∗ map] k↦y ∈ regs, k ↣ᵣ y)
    ={Ep}=∗ ∃ retv regs' mem', ⌜ Store_spec regs r1 r2 regs' mem mem' retv⌝ ∗
-                           ⤇ fill K (of_val retv) ∗ ([∗ map] a↦w ∈ mem', a ↣ₐ w) ∗ [∗ map] k↦y ∈ regs', k ↣ᵣ y.
-  Proof.
-    iIntros (Hinstr Hvpc HPC Dregs Hmem_pc HaStore Hnclose) "(Hinv & Hj & >Hmem & >Hmap)".
+                           ⤇ fill K (of_val retv) ∗ ([∗ map] (a:PhysAddr)↦w ∈ mem', a ↣ₐ w) ∗ [∗ map] k↦y ∈ regs', k ↣ᵣ y.
+  Proof. Admitted.
+    (* iIntros (Hinstr Hvpc HPC Dregs Hmem_pc HaStore Hnclose) "(Hinv & Hj & >Hmem & >Hmap)".
     iDestruct "Hinv" as (ρ) "Hinv". rewrite /spec_inv.
     iInv specN as ">Hinv'" "Hclose". iDestruct "Hinv'" as (e [σr σm]) "[Hown %] /=".
     iDestruct (regspec_heap_valid_inclSepM with "Hown Hmap") as %Hregs.
@@ -45,7 +45,7 @@ Section cap_lang_spec_rules.
     pose proof (lookup_weaken _ _ _ _ HPC Hregs).
     specialize (indom_regs_incl _ _ _ Dregs Hregs) as Hri. unfold regs_of in Hri.
     odestruct (Hri r1) as [r1v [Hr'1 Hr1]]. by set_solver+.
-    iDestruct (memspec_heap_valid_inSepM _ _ _ _ pc_a with "Hown Hmem") as %Hma; eauto.
+    iDestruct (memspec_heap_valid_inSepM _ _ _ _ (TEMP_virt_to_phys pc_a) with "Hown Hmem") as %Hma; eauto.
     iDestruct (spec_expr_valid with "[$Hown $Hj]") as %Heq; subst e.
     specialize (normal_always_step (σr,σm)) as [c [ σ2 Hstep]].
     eapply step_exec_inv in Hstep; eauto.
@@ -92,7 +92,7 @@ Section cap_lang_spec_rules.
      pose proof (allow_store_implies_storev r1 r2 mem regs p b e a storev) as (oldv & Hmema); auto.
 
      (* Given this, prove that a is also present in the memory itself *)
-     iDestruct (memspec_v_implies_m_v mem (σr,σm) _ b e a oldv with "Hmem Hown" ) as %Hma' ; auto.
+     iDestruct (memspec_v_implies_m_v mem (σr,σm) _ (TEMP_virt_to_phys b) (TEMP_virt_to_phys e) (TEMP_virt_to_phys a) oldv with "Hmem Hown" ) as %Hma' ; auto.
 
     destruct (incrementPC regs ) as [ regs' |] eqn:Hregs'.
     2: { (* Failure: the PC could not be incremented correctly *)
@@ -107,7 +107,7 @@ Section cap_lang_spec_rules.
       iPureIntro. eapply Store_spec_failure_store; eauto. by constructor.
     }
 
-    iMod ((memspec_heap_update_inSepM _ _ _ a storev) with "Hown Hmem") as "[Hown Hmem]"; eauto.
+    iMod ((memspec_heap_update_inSepM _ _ _ (TEMP_virt_to_phys a) storev) with "Hown Hmem") as "[Hown Hmem]"; eauto.
 
      (* Success *)
     rewrite /update_mem /= in Hstep.
@@ -125,30 +125,30 @@ Section cap_lang_spec_rules.
     iPureIntro. eapply Store_spec_success; eauto.
       * split; auto. exact Hr'1. all: auto.
       * unfold incrementPC. rewrite a_pc1 HPC''. auto.
-  Qed.
+  Qed. *)
 
   Lemma step_store_success_reg E K pc_p pc_b pc_e pc_a pc_a' w dst src w'
          p b e a w'' :
       decodeInstrW w = Store dst (inr src) →
      isCorrectPC (WCap pc_p pc_b pc_e pc_a) →
-     (pc_a + 1)%a = Some pc_a' →
+     (pc_a + 1)%va = Some pc_a' →
      writeAllowed p = true ∧ withinBoundsVirt b e a = true →
      nclose specN ⊆ E →
 
      spec_ctx ∗ ⤇ fill K (Instr Executable)
               ∗  ▷ PC ↣ᵣ WCap pc_p pc_b pc_e pc_a
-              ∗ ▷ pc_a ↣ₐ w
+              ∗ ▷ (TEMP_virt_to_phys pc_a) ↣ₐ w
               ∗ ▷ src ↣ᵣ w''
               ∗ ▷ dst ↣ᵣ WCap p b e a
-              ∗ ▷ a ↣ₐ w'
+              ∗ ▷ (TEMP_virt_to_phys a) ↣ₐ w'
      ={E}=∗ ⤇ fill K (Instr NextI)
          ∗ PC ↣ᵣ WCap pc_p pc_b pc_e pc_a'
-         ∗ pc_a ↣ₐ w
+         ∗ (TEMP_virt_to_phys pc_a) ↣ₐ w
          ∗ src ↣ᵣ w''
          ∗ dst ↣ᵣ WCap p b e a
-         ∗ a ↣ₐ w''.
-  Proof.
-    iIntros (Hinstr Hvpc Hpca' [Hwa Hwb] Hnclose)
+         ∗ (TEMP_virt_to_phys a) ↣ₐ w''.
+  Proof. Admitted.
+    (* iIntros (Hinstr Hvpc Hpca' [Hwa Hwb] Hnclose)
             "(Hown & Hj & >HPC & >Hi & >Hsrc & >Hdst & >Hsrca)".
     iDestruct (rules_binary_base.map_of_regs_3 with "HPC Hsrc Hdst") as "[Hmap (%&%&%)]".
     iDestruct (spec_memMap_resource_2ne_apply with "Hi Hsrca") as "[Hmem %]"; auto.
@@ -172,28 +172,28 @@ Section cap_lang_spec_rules.
        destruct X; try incrementPC_inv; simplify_map_eq; eauto.
        destruct o. all: try congruence.
      }
-    Qed.
+    Qed. *)
 
   Lemma step_store_success_z E K pc_p pc_b pc_e pc_a pc_a' w dst z w'
          p b e a :
      decodeInstrW w = Store dst (inl z) →
      isCorrectPC (WCap pc_p pc_b pc_e pc_a) →
-     (pc_a + 1)%a = Some pc_a' →
+     (pc_a + 1)%va = Some pc_a' →
      writeAllowed p = true ∧ withinBoundsVirt b e a = true →
      nclose specN ⊆ E →
 
      spec_ctx ∗ ⤇ fill K (Instr Executable)
               ∗ ▷ PC ↣ᵣ WCap pc_p pc_b pc_e pc_a
-              ∗ ▷ pc_a ↣ₐ w
+              ∗ ▷ (TEMP_virt_to_phys pc_a) ↣ₐ w
               ∗ ▷ dst ↣ᵣ WCap p b e a
-              ∗ ▷ a ↣ₐ w'
+              ∗ ▷ (TEMP_virt_to_phys a) ↣ₐ w'
      ={E}=∗ ⤇ fill K (Instr NextI)
          ∗ PC ↣ᵣ WCap pc_p pc_b pc_e pc_a'
-         ∗ pc_a ↣ₐ w
+         ∗ (TEMP_virt_to_phys pc_a) ↣ₐ w
          ∗ dst ↣ᵣ WCap p b e a
-         ∗ a ↣ₐ WInt z.
-  Proof.
-    iIntros (Hinstr Hvpc Hpca' [Hwa Hwb] Hnclose)
+         ∗ (TEMP_virt_to_phys a) ↣ₐ WInt z.
+  Proof. Admitted.
+    (* iIntros (Hinstr Hvpc Hpca' [Hwa Hwb] Hnclose)
             "(Hown & Hj & >HPC & >Hi & >Hdst & >Hsrca)".
     iDestruct (rules_binary_base.map_of_regs_2 with "HPC Hdst") as "[Hmap %]".
     iDestruct (spec_memMap_resource_2ne_apply with "Hi Hsrca") as "[Hmem %]"; auto.
@@ -218,6 +218,6 @@ Section cap_lang_spec_rules.
        destruct X; try incrementPC_inv; simplify_map_eq; eauto.
        destruct o. all: try congruence.
      }
-  Qed.
+  Qed. *)
 
 End cap_lang_spec_rules.
